tests/blake2b-32-test-streaming.c
@@ -17,9 +17,7 @@
 
 typedef struct Hacl_Streaming_Blake2_blake2b_32_state_s blake2_state;
 
-int
-main()
-{
+int main() {
   bool ok = true;
 
   // Here, I can't really loop over the vectors... because I want to exercise
@@ -29,9 +27,9 @@ main()
   uint8_t tag[64] = {};
   // Use only the vectors without keys: streaming blake2 in keyed mode is not
   // implemented.
-  blake2_test_vector* v = &vectors2b[2];
+  blake2_test_vector *v = &vectors2b[2];
 
-  blake2_state* s = Hacl_Streaming_Blake2_blake2b_32_no_key_create_in();
+  blake2_state *s = Hacl_Streaming_Blake2_blake2b_32_no_key_malloc();
   assert(Hacl_Streaming_Blake2_blake2b_32_no_key_update(s, NULL, 0) == 0);
   assert(Hacl_Streaming_Blake2_blake2b_32_no_key_update(s, v->input, 8) == 0);
   assert(Hacl_Streaming_Blake2_blake2b_32_no_key_update(s, v->input + 8, 8) ==
@@ -39,12 +37,12 @@ main()
   assert(Hacl_Streaming_Blake2_blake2b_32_no_key_update(s, v->input + 16, 16) ==
          0);
   assert(Hacl_Streaming_Blake2_blake2b_32_no_key_update(
-           s, v->input + 32, v->input_len - 32) == 0);
-  Hacl_Streaming_Blake2_blake2b_32_no_key_finish(s, tag);
+             s, v->input + 32, v->input_len - 32) == 0);
+  Hacl_Streaming_Blake2_blake2b_32_no_key_digest(s, tag);
   ok &= compare_and_print(64, tag, v->expected);
 
   v++;
-  Hacl_Streaming_Blake2_blake2b_32_no_key_init(s);
+  Hacl_Streaming_Blake2_blake2b_32_no_key_reset(s);
   assert(Hacl_Streaming_Blake2_blake2b_32_no_key_update(s, NULL, 0) == 0);
   assert(Hacl_Streaming_Blake2_blake2b_32_no_key_update(s, v->input, 8) == 0);
   assert(Hacl_Streaming_Blake2_blake2b_32_no_key_update(s, v->input + 8, 8) ==
@@ -54,8 +52,8 @@ main()
   assert(Hacl_Streaming_Blake2_blake2b_32_no_key_update(s, v->input + 32, 32) ==
          0);
   assert(Hacl_Streaming_Blake2_blake2b_32_no_key_update(
-           s, v->input + 64, v->input_len - 64) == 0);
-  Hacl_Streaming_Blake2_blake2b_32_no_key_finish(s, tag);
+             s, v->input + 64, v->input_len - 64) == 0);
+  Hacl_Streaming_Blake2_blake2b_32_no_key_digest(s, tag);
   ok &= compare_and_print(64, tag, v->expected);
 
   Hacl_Streaming_Blake2_blake2b_32_no_key_free(s);
