tests/blake2s-32-test-streaming.c
@@ -31,23 +31,23 @@ main()
   // implemented.
   blake2_test_vector* v = &vectors2s[5];
 
-  blake2_state* s = Hacl_Streaming_Blake2_blake2s_32_no_key_create_in();
+  blake2_state* s = Hacl_Streaming_Blake2_blake2s_32_no_key_malloc();
   assert(Hacl_Streaming_Blake2_blake2s_32_no_key_update(s, NULL, 0) == 0);
   assert(Hacl_Streaming_Blake2_blake2s_32_no_key_update(
            s, v->input, v->input_len) == 0);
-  Hacl_Streaming_Blake2_blake2s_32_no_key_finish(s, tag);
+  Hacl_Streaming_Blake2_blake2s_32_no_key_digest(s, tag);
   ok &= compare_and_print(32, tag, v->expected);
 
   v++;
-  Hacl_Streaming_Blake2_blake2s_32_no_key_init(s);
+  Hacl_Streaming_Blake2_blake2s_32_no_key_reset(s);
   assert(Hacl_Streaming_Blake2_blake2s_32_no_key_update(s, NULL, 0) == 0);
   assert(Hacl_Streaming_Blake2_blake2s_32_no_key_update(
            s, v->input, v->input_len) == 0);
-  Hacl_Streaming_Blake2_blake2s_32_no_key_finish(s, tag);
+  Hacl_Streaming_Blake2_blake2s_32_no_key_digest(s, tag);
   ok &= compare_and_print(32, tag, v->expected);
 
   v++;
-  Hacl_Streaming_Blake2_blake2s_32_no_key_init(s);
+  Hacl_Streaming_Blake2_blake2s_32_no_key_reset(s);
   assert(Hacl_Streaming_Blake2_blake2s_32_no_key_update(s, NULL, 0) == 0);
   assert(Hacl_Streaming_Blake2_blake2s_32_no_key_update(s, v->input, 8) == 0);
   assert(Hacl_Streaming_Blake2_blake2s_32_no_key_update(s, v->input + 8, 8) ==
@@ -60,11 +60,11 @@ main()
          0);
   assert(Hacl_Streaming_Blake2_blake2s_32_no_key_update(
            s, v->input + 128, 127) == 0);
-  Hacl_Streaming_Blake2_blake2s_32_no_key_finish(s, tag);
+  Hacl_Streaming_Blake2_blake2s_32_no_key_digest(s, tag);
   ok &= compare_and_print(32, tag, v->expected);
 
   v++;
-  Hacl_Streaming_Blake2_blake2s_32_no_key_init(s);
+  Hacl_Streaming_Blake2_blake2s_32_no_key_reset(s);
   assert(Hacl_Streaming_Blake2_blake2s_32_no_key_update(s, NULL, 0) == 0);
   assert(Hacl_Streaming_Blake2_blake2s_32_no_key_update(s, v->input, 8) == 0);
   assert(Hacl_Streaming_Blake2_blake2s_32_no_key_update(s, v->input + 8, 8) ==
@@ -77,11 +77,11 @@ main()
          0);
   assert(Hacl_Streaming_Blake2_blake2s_32_no_key_update(
            s, v->input + 128, v->input_len - 128) == 0);
-  Hacl_Streaming_Blake2_blake2s_32_no_key_finish(s, tag);
+  Hacl_Streaming_Blake2_blake2s_32_no_key_digest(s, tag);
   ok &= compare_and_print(32, tag, v->expected);
 
   v++;
-  Hacl_Streaming_Blake2_blake2s_32_no_key_init(s);
+  Hacl_Streaming_Blake2_blake2s_32_no_key_reset(s);
   assert(Hacl_Streaming_Blake2_blake2s_32_no_key_update(s, NULL, 0) == 0);
   assert(Hacl_Streaming_Blake2_blake2s_32_no_key_update(s, v->input, 8) == 0);
   assert(Hacl_Streaming_Blake2_blake2s_32_no_key_update(s, v->input + 8, 8) ==
@@ -90,7 +90,7 @@ main()
          0);
   assert(Hacl_Streaming_Blake2_blake2s_32_no_key_update(
            s, v->input + 32, v->input_len - 32) == 0);
-  Hacl_Streaming_Blake2_blake2s_32_no_key_finish(s, tag);
+  Hacl_Streaming_Blake2_blake2s_32_no_key_digest(s, tag);
   ok &= compare_and_print(32, tag, v->expected);
 
   Hacl_Streaming_Blake2_blake2s_32_no_key_free(s);
