tests/sha3-streaming-test.c
@@ -10,10 +10,10 @@ const uint8_t expected_hash[] = { 0x64, 0x4b, 0xcc, 0x7e, 0x56, 0x43, 0x73,
 int
 main()
 {
-  Hacl_Streaming_SHA3_state_256* s = Hacl_Streaming_SHA3_create_in_256();
+  Hacl_Streaming_SHA3_state_256* s = Hacl_Streaming_SHA3_malloc_256();
   assert(Hacl_Streaming_SHA3_update_256(s, (uint8_t*)"hello world", 11) == 0);
   uint8_t hash[32] = { 0 };
-  Hacl_Streaming_SHA3_finish_256(s, hash);
+  Hacl_Streaming_SHA3_digest_256(s, hash);
   Hacl_Streaming_SHA3_free_256(s);
   for (int i = 0; i < 32; ++i) {
     if (hash[i] != expected_hash[i]) {
