code/streaming/Hacl.Streaming.Poly1305_256.fst
@@ -14,9 +14,9 @@ let poly1305_256_state = F.state_s (poly1305 M256) () (t M256) (k.I.s ())
 
 noextract
 let alloca = F.alloca (poly1305 M256) () (t M256) (k.I.s ())
-let create_in = F.create_in (poly1305 M256) () (t M256) (k.I.s ())
-let init = F.init (poly1305 M256) (G.hide ()) (t M256) (k.I.s ())
+let malloc = F.malloc (poly1305 M256) () (t M256) (k.I.s ())
+let reset = F.reset (poly1305 M256) (G.hide ()) (t M256) (k.I.s ())
 [@@ Comment "0 = success, 1 = max length exceeded" ]
 let update = F.update (poly1305 M256) (G.hide ()) (t M256) (k.I.s ())
-let finish = F.mk_finish (poly1305 M256) () (t M256) (k.I.s ())
+let digest = F.digest (poly1305 M256) () (t M256) (k.I.s ())
 let free = F.free (poly1305 M256) (G.hide ()) (t M256) (k.I.s ())
