code/ed25519/Hacl.Impl.SHA512.ModQ.fst
@@ -35,7 +35,7 @@ let sha512_pre_msg hash prefix len input =
   let st = Hash.alloca_512 () in
   let _ = Hash.update_512 st prefix 32ul in
   let _ = Hash.update_512 st input len in
-  Hash.finish_512 st hash;
+  Hash.digest_512 st hash;
   let h1 = ST.get () in
   assert (as_seq h1 hash == Spec.Agile.Hash.hash Spec.Hash.Definitions.SHA2_512
     (Seq.append (Seq.append (Seq.empty) (as_seq h0 prefix)) (as_seq h0 input)));
@@ -65,7 +65,7 @@ let sha512_pre_pre2_msg hash prefix prefix2 len input =
   let _ = Hash.update_512 st prefix 32ul in
   let _ = Hash.update_512 st prefix2 32ul in
   let _ = Hash.update_512 st input len in
-  Hash.finish_512 st hash;
+  Hash.digest_512 st hash;
   Seq.append_empty_l (as_seq h0 prefix);
   pop_frame ()
 
