code/streaming/Hacl.Streaming.SHA2.fst
@@ -67,7 +67,7 @@ let alloca_256 = F.alloca hacl_sha2_256 () (state_t_256.s ()) (G.erased unit)
 [@@ Comment
 "Allocate initial state for the SHA2_256 hash. The state is to be freed by
 calling `free_256`."]
-let create_in_256 = F.create_in hacl_sha2_256 () (state_t_256.s ()) (G.erased unit)
+let malloc_256 = F.malloc hacl_sha2_256 () (state_t_256.s ()) (G.erased unit)
 
 [@@ Comment
 "Copies the state passed as argument into a newly allocated state (deep copy).
@@ -78,7 +78,7 @@ let copy_256 = F.copy hacl_sha2_256 () (state_t_256.s ()) (G.erased unit)
 
 [@@ Comment
 "Reset an existing state to the initial hash state with empty data."]
-let init_256 = F.init hacl_sha2_256 (G.hide ()) (state_t_256.s ()) (G.erased unit)
+let reset_256 = F.reset hacl_sha2_256 (G.hide ()) (state_t_256.s ()) (G.erased unit)
 
 [@@ CInline ]
 private
@@ -87,21 +87,21 @@ let update_224_256 = F.update hacl_sha2_256 (G.hide ()) (state_t_256.s ()) (G.er
 [@@ Comment
 "Feed an arbitrary amount of data into the hash. This function returns 0 for
 success, or 1 if the combined length of all of the data passed to `update_256`
-(since the last call to `init_256`) exceeds 2^61-1 bytes.
+(since the last call to `reset_256`) exceeds 2^61-1 bytes.
 
 This function is identical to the update function for SHA2_224.";
 ]
 let update_256: F.update_st hacl_sha2_256 (G.hide ()) (state_t_256.s ()) (G.erased unit) = fun p input input_len -> update_224_256 p input input_len
 
 [@@ Comment
-"Write the resulting hash into `dst`, an array of 32 bytes. The state remains
-valid after a call to `finish_256`, meaning the user may feed more data into
-the hash via `update_256`. (The finish_256 function operates on an internal copy of
+"Write the resulting hash into `output`, an array of 32 bytes. The state remains
+valid after a call to `digest_256`, meaning the user may feed more data into
+the hash via `update_256`. (The digest_256 function operates on an internal copy of
 the state and therefore does not invalidate the client-held state `p`.)"]
-let finish_256 = F.mk_finish hacl_sha2_256 () (state_t_256.s ()) (G.erased unit)
+let digest_256 = F.digest hacl_sha2_256 () (state_t_256.s ()) (G.erased unit)
 
 [@@ Comment
-"Free a state allocated with `create_in_256`.
+"Free a state allocated with `malloc_256`.
 
 This function is identical to the free function for SHA2_224."]
 let free_256 = F.free hacl_sha2_256 (G.hide ()) (state_t_256.s ()) (G.erased unit)
@@ -126,16 +126,16 @@ let sha256 input input_len dst =
 
 inline_for_extraction noextract
 let alloca_224 = F.alloca hacl_sha2_224 () (state_t_224.s ()) (G.erased unit)
-let create_in_224 = F.create_in hacl_sha2_224 () (state_t_224.s ()) (G.erased unit)
-let init_224 = F.init hacl_sha2_224 (G.hide ()) (state_t_224.s ()) (G.erased unit)
+let malloc_224 = F.malloc hacl_sha2_224 () (state_t_224.s ()) (G.erased unit)
+let reset_224 = F.reset hacl_sha2_224 (G.hide ()) (state_t_224.s ()) (G.erased unit)
 // We assume verified clients will rely on Spec.SHA2.Lemmas to prove that update_224 has the same effect as update_256.
 let update_224: F.update_st hacl_sha2_256 (G.hide ()) (state_t_256.s ()) (G.erased unit) = fun p input input_len -> update_224_256 p input input_len
 
 [@@ Comment
-"Write the resulting hash into `dst`, an array of 28 bytes. The state remains
-valid after a call to `finish_224`, meaning the user may feed more data into
+"Write the resulting hash into `output`, an array of 28 bytes. The state remains
+valid after a call to `digest_224`, meaning the user may feed more data into
 the hash via `update_224`."]
-let finish_224 = F.mk_finish hacl_sha2_224 () (state_t_224.s ()) (G.erased unit)
+let digest_224 = F.digest hacl_sha2_224 () (state_t_224.s ()) (G.erased unit)
 let free_224: F.free_st hacl_sha2_256 (G.hide ()) (state_t_256.s ()) (G.erased unit) = fun p -> free_256 p
 
 [@@ Comment
@@ -158,7 +158,7 @@ let sha224 input input_len dst =
 
 inline_for_extraction noextract
 let alloca_512 = F.alloca hacl_sha2_512 () (state_t_512.s ()) (G.erased unit)
-let create_in_512 = F.create_in hacl_sha2_512 () (state_t_512.s ()) (G.erased unit)
+let malloc_512 = F.malloc hacl_sha2_512 () (state_t_512.s ()) (G.erased unit)
 
 [@@ Comment
 "Copies the state passed as argument into a newly allocated state (deep copy).
@@ -167,7 +167,7 @@ useful, for instance, if your control-flow diverges and you need to feed
 more (different) data into the hash in each branch."]
 let copy_512 = F.copy hacl_sha2_512 () (state_t_512.s ()) (G.erased unit)
 
-let init_512 = F.init hacl_sha2_512 (G.hide ()) (state_t_512.s ()) (G.erased unit)
+let reset_512 = F.reset hacl_sha2_512 (G.hide ()) (state_t_512.s ()) (G.erased unit)
 
 [@@ CInline ]
 private
@@ -175,21 +175,21 @@ let update_384_512 = F.update hacl_sha2_512 (G.hide ()) (state_t_512.s ()) (G.er
 [@@ Comment
 "Feed an arbitrary amount of data into the hash. This function returns 0 for
 success, or 1 if the combined length of all of the data passed to `update_512`
-(since the last call to `init_512`) exceeds 2^125-1 bytes.
+(since the last call to `reset_512`) exceeds 2^125-1 bytes.
 
 This function is identical to the update function for SHA2_384.";
 ]
 let update_512: F.update_st hacl_sha2_512 (G.hide ()) (state_t_512.s ()) (G.erased unit) = fun p input input_len -> update_384_512 p input input_len
 
 [@@ Comment
-"Write the resulting hash into `dst`, an array of 64 bytes. The state remains
-valid after a call to `finish_512`, meaning the user may feed more data into
-the hash via `update_512`. (The finish_512 function operates on an internal copy of
+"Write the resulting hash into `output`, an array of 64 bytes. The state remains
+valid after a call to `digest_512`, meaning the user may feed more data into
+the hash via `update_512`. (The digest_512 function operates on an internal copy of
 the state and therefore does not invalidate the client-held state `p`.)"]
-let finish_512 = F.mk_finish hacl_sha2_512 () (state_t_512.s ()) (G.erased unit)
+let digest_512 = F.digest hacl_sha2_512 () (state_t_512.s ()) (G.erased unit)
 
 [@@ Comment
-"Free a state allocated with `create_in_512`.
+"Free a state allocated with `malloc_512`.
 
 This function is identical to the free function for SHA2_384.";
 ]
@@ -215,15 +215,15 @@ let sha512 input input_len dst =
 
 inline_for_extraction noextract
 let alloca_384 = F.alloca hacl_sha2_384 () (state_t_384.s ()) (G.erased unit)
-let create_in_384 = F.create_in hacl_sha2_384 () (state_t_384.s ()) (G.erased unit)
-let init_384 = F.init hacl_sha2_384 (G.hide ()) (state_t_384.s ()) (G.erased unit)
+let malloc_384 = F.malloc hacl_sha2_384 () (state_t_384.s ()) (G.erased unit)
+let reset_384 = F.reset hacl_sha2_384 (G.hide ()) (state_t_384.s ()) (G.erased unit)
 let update_384: F.update_st hacl_sha2_512 (G.hide ()) (state_t_512.s ()) (G.erased unit) = fun p input input_len -> update_384_512 p input input_len
 
 [@@ Comment
-"Write the resulting hash into `dst`, an array of 48 bytes. The state remains
-valid after a call to `finish_384`, meaning the user may feed more data into
+"Write the resulting hash into `output`, an array of 48 bytes. The state remains
+valid after a call to `digest_384`, meaning the user may feed more data into
 the hash via `update_384`."]
-let finish_384 = F.mk_finish hacl_sha2_384 () (state_t_384.s ()) (G.erased unit)
+let digest_384 = F.digest hacl_sha2_384 () (state_t_384.s ()) (G.erased unit)
 
 let free_384: F.free_st hacl_sha2_512 (G.hide ()) (state_t_512.s ()) (G.erased unit) = fun p -> free_512 p
 
